Rewrite general bloom filter by functions defined in ConFilter.

examples/sbf/general_bf.v
@@ -3,81 +3,91 @@ Require Import Coq.ZArith.ZArith.
 Require Import Coq.Lists.List.
 Require Import Coq.Logic.FunctionalExtensionality.
 Require Import ProD3.examples.sbf.Utils.
+Require Import ProD3.examples.sbf.ConFilter.
 
 Section BLOOM_FILTER.
 
   (* Number of hashes *)
-  Context {Index: Type}.
+  Definition Index := Z.
 
-  Parameter index_eqb: Index -> Index -> bool.
+  Definition index_eqb: Index -> Index -> bool := Z.eqb.
 
-  Parameter index_refl: forall i, index_eqb i i = true.
+  Lemma index_refl: forall i, index_eqb i i = true.
+  Proof. apply Z.eqb_refl. Qed.
 
   Definition HashFunc := Z -> Index.
 
-  Definition Filter := Index -> bool.
+  Definition add_hash (z: Z) (h: HashFunc) (F: row) :=
+    row_insert F (h z).
 
-  Definition upd (F: Filter) (i:Index) (b:bool): Filter :=
-    fun j => if index_eqb i j then b else F j.
+  Definition add (hashes: list HashFunc) (fs: frame) (z: Z) : frame :=
+    frame_insert fs (map (fun hash => hash z) hashes).
 
-  Definition get (F: Filter) (i: Index): bool := F i.
-
-  Definition add_hash (z: Z) (h: HashFunc) (F: Filter) := upd F (h z) true.
-
-  Definition add (hashes: list HashFunc) (fs: list Filter) (z: Z) : list Filter :=
-    map2 (add_hash z) hashes fs.
-
-  Definition addm (hashes: list HashFunc) (fs: list Filter) (zs: list Z) :=
+  Definition addm (hashes: list HashFunc) (fs: frame) (zs: list Z) :=
     List.fold_left (add hashes) zs fs.
 
-  Definition query (hashes: list HashFunc) (fs: list Filter) (z: Z): bool :=
-    List.fold_left andb (map2 (fun h f => get f (h z)) hashes fs) true.
+  Definition query (hashes: list HashFunc) (fs: frame) (z: Z): bool :=
+    frame_query fs (map (fun hash => hash z) hashes).
 
-  Lemma bf_add_get_true: forall z h a, get (add_hash z h a) (h z) = true.
+  Definition hash_row_compatible (h: HashFunc) (r: row): Prop :=
+    forall x, 0 <= h x < Zlength r.
+
+  Lemma bf_add_get_true: forall z h a,
+      hash_row_compatible h a ->
+      row_query (add_hash z h a) (h z) = true.
   Proof.
-    unfold get, add_hash. intros. unfold upd. rewrite index_refl. easy.
+    unfold row_query, add_hash, row_insert. intros.
+    rewrite upd_Znth_same; auto.
   Qed.
 
   Lemma add_hash_comm: forall x y f h,
       add_hash x h (add_hash y h f) = add_hash y h (add_hash x h f).
   Proof.
-    unfold add_hash, upd. intros.
-    apply functional_extensionality. intros z.
-    destruct (index_eqb (h x) z);
-    destruct (index_eqb (h y) z); auto.
-  Qed.
-
-  Lemma add_comm x y fs hashes:
-    length fs = length hashes -> add hashes (add hashes fs x) y = add hashes (add hashes fs y) x.
-  Proof.
-    intros. revert fs hashes H. induction fs; intros; simpl; unfold add; destruct hashes.
-    - unfold map2. now simpl.
-    - simpl in H; inversion H.
-    - simpl in H; inversion H.
-    - rewrite !map2_cons. rewrite add_hash_comm. f_equal.
-      unfold add in IHfs. apply IHfs. now inversion H.
-  Qed.
-
-  Lemma bf_add_query_true: forall fs hashes z,
-      length fs = length hashes -> query hashes (add hashes fs z) z = true.
-  Proof.
-    induction fs; intros; simpl; unfold add, query; destruct hashes.
-    - now simpl.
-    - simpl in H; inversion H.
-    - simpl in H; inversion H.
-    - rewrite !map2_cons. simpl in H. inversion H. clear H.
-      specialize (IHfs _ z H1). unfold add, query in IHfs.
-      rewrite bf_add_get_true. simpl fold_left. apply IHfs.
+    unfold add_hash, row_insert. intros.
+    list_solve.
   Qed.
 
   Lemma add_cons: forall h hs f fs z, add (h :: hs) (f :: fs) z = add_hash z h f :: add hs fs z.
-  Proof. intros. unfold add. apply map2_cons. Qed.
+  Proof. intros. unfold add, add_hash, frame_insert. apply map2_cons. Qed.
+
+  Lemma add_comm x y fs hashes:
+    length fs = length hashes ->
+    add hashes (add hashes fs x) y = add hashes (add hashes fs y) x.
+  Proof.
+    intros. revert fs hashes H. induction fs; intros; simpl; destruct hashes.
+    - now simpl.
+    - simpl in H; inversion H.
+    - simpl in H; inversion H.
+    - rewrite !add_cons. rewrite add_hash_comm. f_equal.
+      apply IHfs. now inversion H.
+  Qed.
+
+  Lemma query_cons: forall h hashes f fs z,
+      query (h :: hashes) (f :: fs) z = (row_query f (h z) && query hashes fs z)%bool.
+  Proof.
+    intros. unfold query. simpl. unfold frame_query. unfold fold_andb.
+    rewrite map2_cons. simpl. destruct (row_query f (h z)); simpl; auto.
+    now rewrite fold_andb_false.
+  Qed.
+
+  Lemma bf_add_query_true: forall fs hashes z,
+      Forall2 hash_row_compatible hashes fs ->
+      query hashes (add hashes fs z) z = true.
+  Proof.
+    induction fs; intros; simpl; destruct hashes.
+    - now simpl.
+    - simpl in H; inversion H.
+    - simpl in H; inversion H.
+    - rewrite add_cons. rewrite query_cons. inversion H. subst. clear H.
+      rewrite IHfs; auto. rewrite Bool.andb_true_r.
+      apply bf_add_get_true; auto.
+  Qed.
 
   Lemma add_length: forall hashes fs z,
       length fs = length hashes -> length (add hashes fs z) = length fs.
   Proof.
-    intros. unfold add, map2. rewrite map_length. rewrite combine_length.
-    rewrite H. rewrite Nat.min_id. easy.
+    intros. unfold add, frame_insert, map2. rewrite map_length, combine_length.
+    rewrite map_length, H. rewrite Nat.min_id. easy.
   Qed.
 
   Lemma addm_length: forall hashes fs zs,
@@ -100,12 +110,38 @@ Section BLOOM_FILTER.
       rewrite addm_length; auto.
   Qed.
 
+  Lemma hash_row_compatible_add_hash:
+    forall (z : Z) (x : HashFunc) (y : row),
+      hash_row_compatible x y -> hash_row_compatible x (add_hash z x y).
+  Proof.
+    unfold hash_row_compatible. intros. unfold add_hash, row_insert.
+    now rewrite Zlength_upd_Znth.
+  Qed.
+
+  Lemma hash_row_compatible_add: forall hashes fs z,
+      Forall2 hash_row_compatible hashes fs ->
+      Forall2 hash_row_compatible hashes (add hashes fs z).
+  Proof.
+    intros. induction H.
+    - unfold add, frame_insert, map2. simpl. constructor.
+    - rewrite add_cons. constructor; auto. now apply hash_row_compatible_add_hash.
+  Qed.
+
+  Lemma hash_row_compatible_addm:
+    forall (zs : list Z) (fs : list row) (hashes : list HashFunc),
+      Forall2 hash_row_compatible hashes fs ->
+      Forall2 hash_row_compatible hashes (addm hashes fs zs).
+  Proof.
+    induction zs; intros; simpl; auto.
+    apply IHzs. now apply hash_row_compatible_add.
+  Qed.
+
   Theorem BFNoFalseNegative: forall z zs fs hashes,
-      length fs = length hashes ->
+      Forall2 hash_row_compatible hashes fs ->
       query hashes (addm hashes (add hashes fs z) zs) z  = true.
   Proof.
-    intros. rewrite addm_add_comm; auto. apply bf_add_query_true.
-    rewrite addm_length; auto.
+    intros. pose proof (Forall2_length H). rewrite addm_add_comm; auto.
+    apply bf_add_query_true. now apply hash_row_compatible_addm.
   Qed.
 
 End BLOOM_FILTER.
